test.v
@@ -1,29 +1,26 @@
 From Minirust.def Require Import ty encoding int_encoding utils.
-Require Import Coq.Init.Byte List NArith ZArith.
+Require Import Coq.Init.Byte List NArith ZArith Lia.
 Import ListNotations.
 
-Record Assumptions := {
- A_PTR_SIZE : PTR_SIZE = 8;
- A_ENDIANNESS : ENDIANNESS = BigEndian;
- A_P : P = nat;
+Lemma ptr_size_gt0 : 8 > 0. lia. Qed.
+
+Local Instance TestParams : Params := {
+  PTR_SIZE := 8;
+  ENDIANNESS := BigEndian;
+  P := nat;
+  P_EQ := Nat.eqb;
+  P_EQ_REFLECT := Nat.eqb_spec;
+  PTR_SIZE_GT0 := ptr_size_gt0;
 }.
 
-Lemma prov (A: Assumptions) (n: nat) : P.
-rewrite (A_P A).
-apply n.
-Qed.
-
-Ltac exec A := repeat (
+Ltac exec := repeat (
   simpl ||
   auto ||
   split ||
-  unfold encode,encode_int,decode_int,decode_int_raw,encode_int_raw,encode_array,decode_array ||
-  rewrite (A_PTR_SIZE A) ||
-  rewrite (A_ENDIANNESS A) ||
-  rewrite (A_P A)
+  unfold encode,encode_int,decode_int,decode_int_raw,encode_int_raw,encode_array,decode_array
 ).
 
-Lemma test_int (A : Assumptions) :
+Lemma test_int :
 (* encode *)
 (encode (TInt 1 Unsigned) (VInt 255%Z)) = Some [Init "255" None] /\
 (encode (TInt 2 Signed) (VInt (-1)%Z)) = Some [Init "255" None; Init "255" None] /\
@@ -33,13 +30,13 @@ Lemma test_int (A : Assumptions) :
 (* decode *)
 (decode (TInt 2 Unsigned) [Init "000" None; Init "001" None]) = Some (VInt 1%Z) /\
 (decode (TInt 2 Unsigned) [Init "001" None; Init "000" None]) = Some (VInt 256%Z) /\
-(decode (TInt 2 Unsigned) [Init "000" (Some (prov A 12)); Init "000" None]) = Some (VInt 0%Z) /\
+(decode (TInt 2 Unsigned) [Init "000" (Some 12); Init "000" None]) = Some (VInt 0%Z) /\
 
 (* error *)
 (decode (TInt 2 Unsigned) [Init "000" None]) = None.
-Proof. exec A. Qed.
+Proof. exec. Qed.
 
-Lemma test_bool (A: Assumptions) :
+Lemma test_bool :
 (* encode *)
 (encode TBool (VBool true) = Some [Init "001" None]) /\
 (encode TBool (VBool false) = Some [Init "000" None]) /\
@@ -47,8 +44,8 @@ Lemma test_bool (A: Assumptions) :
 (* decode *)
 (decode TBool [Init "001" None]) = Some (VBool true) /\
 (decode TBool [Init "000" None]) = Some (VBool false) /\
-(decode TBool [Init "001" (Some (prov A 12))]) = Some (VBool true) /\
-(decode TBool [Init "000" (Some (prov A 42))]) = Some (VBool false) /\
+(decode TBool [Init "001" (Some 12)]) = Some (VBool true) /\
+(decode TBool [Init "000" (Some 42)]) = Some (VBool false) /\
 
 (* error *)
 (encode TBool (VInt 12%Z)) = None /\
@@ -56,9 +53,9 @@ Lemma test_bool (A: Assumptions) :
 (decode TBool []) = None /\
 (decode TBool [Init "001" None; Init "001" None]) = None /\
 (decode TBool [Uninit]) = None.
-Proof. exec A. Qed.
+Proof. exec. Qed.
 
-Lemma test_array (A: Assumptions) :
+Lemma test_array :
 (* encode *)
 encode (TArray (TInt 2 Unsigned) 2%Z) (VTuple [VInt 12%Z; VInt 13%Z]) = Some [Init "000" None; Init "012" None; Init "000" None; Init "013" None]  /\
 decode (TArray (TInt 2 Unsigned) 2%Z) [Init "000" None; Init "012" None; Init "000" None; Init "013" None] = Some (VTuple [VInt 12%Z; VInt 13%Z]) /\
@@ -70,4 +67,4 @@ decode (TArray TBool 0%Z) [] = Some (VTuple []) /\
 (* error *)
 encode (TArray TBool 1%Z) (VTuple []) = None /\
 decode (TArray TBool 1%Z) [] = None.
-Proof. exec A. Qed.
+Proof. exec. Qed.
